raft-proofs/VotesLeCurrentTermProof.v
@@ -1,0 +1,96 @@
+Require Import Arith.
+Require Import NPeano.
+Require Import Omega.
+Require Import List.
+Require Import Coq.Numbers.Natural.Abstract.NDiv.
+Import ListNotations.
+Require Import Sorting.Permutation.
+
+Require Import Util.
+Require Import Net.
+Require Import RaftState.
+Require Import Raft.
+Require Import RaftRefinementInterface.
+Require Import CommonTheorems.
+
+Require Import VerdiTactics.
+
+Require Import VotesLeCurrentTermInterface.
+
+Section VotesCorrect.
+  Context {orig_base_params : BaseParams}.
+  Context {one_node_params : OneNodeParams orig_base_params}.
+  Context {raft_params : RaftParams orig_base_params}.
+
+  Context {rri : raft_refinement_interface}.
+
+  Lemma votes_le_current_term_client_request :
+    refined_raft_net_invariant_client_request votes_le_currentTerm.
+  Admitted.
+
+  Lemma votes_le_current_term_timeout :
+    refined_raft_net_invariant_timeout votes_le_currentTerm.
+  Admitted.
+
+  Lemma votes_le_current_term_append_entries :
+    refined_raft_net_invariant_append_entries votes_le_currentTerm.
+  Admitted.
+
+  Lemma votes_le_current_term_append_entries_reply :
+    refined_raft_net_invariant_append_entries_reply votes_le_currentTerm.
+  Admitted.
+
+  Lemma votes_le_current_term_request_vote :
+    refined_raft_net_invariant_request_vote votes_le_currentTerm.
+  Admitted.
+
+  Lemma votes_le_current_term_request_vote_reply :
+    refined_raft_net_invariant_request_vote_reply votes_le_currentTerm.
+  Admitted.
+
+  Lemma votes_le_current_term_do_leader :
+    refined_raft_net_invariant_do_leader votes_le_currentTerm.
+  Admitted.
+
+  Lemma votes_le_current_term_do_generic_server :
+    refined_raft_net_invariant_do_generic_server votes_le_currentTerm.
+  Admitted.
+
+  Lemma votes_le_current_term_state_same_packet_subset :
+    refined_raft_net_invariant_state_same_packet_subset votes_le_currentTerm.
+  Admitted.
+
+  Lemma votes_le_current_term_reboot :
+    refined_raft_net_invariant_reboot votes_le_currentTerm.
+  Admitted.
+
+  Theorem votes_le_current_term_init :
+    refined_raft_net_invariant_init votes_le_currentTerm.
+  Admitted.
+
+  Theorem votes_le_current_term_invariant :
+    forall net,
+      refined_raft_intermediate_reachable net ->
+      votes_le_currentTerm net.
+  Proof.
+    intros.
+    eapply refined_raft_net_invariant; eauto.
+    - apply votes_le_current_term_init.
+    - apply votes_le_current_term_client_request.
+    - apply votes_le_current_term_timeout.
+    - apply votes_le_current_term_append_entries.
+    - apply votes_le_current_term_append_entries_reply.
+    - apply votes_le_current_term_request_vote.
+    - apply votes_le_current_term_request_vote_reply.
+    - apply votes_le_current_term_do_leader.
+    - apply votes_le_current_term_do_generic_server.
+    - apply votes_le_current_term_state_same_packet_subset.
+    - apply votes_le_current_term_reboot.
+  Qed.
+
+  Instance vlcti : votes_le_current_term_interface.
+  Proof.
+    split.
+    auto using votes_le_current_term_invariant.
+  Qed.
+End VotesCorrect.
